Updates.

FOL/Program/LN/Sub.lean
@@ -1,4 +1,6 @@
 import FOL.Program.LN.Formula
+import FOL.Program.LN.OpenClose
+import FOL.Program.LN.Semantics
 import FOL.Tactics
 
 set_option autoImplicit false
@@ -6,7 +8,7 @@ set_option autoImplicit false
 
 namespace LN
 
-open Formula
+open Var Formula
 
 
 def Var.sub_Var (σ : Var → Var) : Var → Var
@@ -20,9 +22,7 @@ def Formula.sub_Var (σ : Var → Var) : Formula → Formula
   | imp_ phi psi => imp_ (phi.sub_Var σ) (psi.sub_Var σ)
   | forall_ x phi => forall_ x (phi.sub_Var σ)
 
-
 --------------------------------------------------
-
 
 def Var.sub_Str (σ : String → String) : Var → Var
   | free_ x => free_ (σ x)
@@ -34,3 +34,138 @@ def Formula.sub_Str (σ : String → String) : Formula → Formula
   | not_ phi => not_ (phi.sub_Str σ)
   | imp_ phi psi => imp_ (phi.sub_Str σ) (psi.sub_Str σ)
   | forall_ x phi => forall_ x (phi.sub_Str σ)
+
+--------------------------------------------------
+
+def str_fun_to_var_fun
+  (σ : String → String) :
+  Var → Var
+  | free_ x => free_ (σ x)
+  | bound_ i => bound_ i
+
+
+lemma SubOpenVar
+  (v : Var)
+  (σ : String → String)
+  (k : ℕ)
+  (y : String)
+  (h1 : σ y = y) :
+  Var.sub_Var (str_fun_to_var_fun σ) (openVar k (free_ y) v) =
+    openVar k (free_ y) (Var.sub_Var (str_fun_to_var_fun σ) v) :=
+  by
+  cases v
+  case _ x =>
+    simp only [openVar]
+    simp only [Var.sub_Var]
+    simp only [str_fun_to_var_fun]
+  case _ i =>
+    simp only [openVar]
+    split
+    case _ c1 =>
+      simp only [Var.sub_Var]
+      simp only [if_pos c1]
+      simp only [str_fun_to_var_fun]
+      simp only [h1]
+    case _ c1 =>
+      simp only [Var.sub_Var]
+      simp only [if_neg c1]
+
+
+lemma SubCloseVar
+  (v : Var)
+  (σ : String → String)
+  (y : String)
+  (k : ℕ)
+  (h1 : σ y = y)
+  (h2 : ∀ (x : String), ¬ y = σ x) :
+  Var.sub_Var (str_fun_to_var_fun σ) (closeVar (free_ y) k v) =
+    closeVar (free_ y) k (Var.sub_Var (str_fun_to_var_fun σ) v) :=
+  by
+  cases v
+  case free_ x =>
+    simp only [closeVar]
+    by_cases c1 : y = x
+    · subst c1
+      simp only [Var.sub_Var]
+      simp only [str_fun_to_var_fun]
+      simp only [h1]
+      simp
+    · simp
+      simp only [if_neg c1]
+      simp only [Var.sub_Var]
+      simp only [str_fun_to_var_fun]
+      specialize h2 x
+      simp only [if_neg h2]
+  case bound_ i =>
+    simp only [closeVar]
+    simp only [Var.sub_Var]
+
+
+lemma SubOpenFormula
+  (F : Formula)
+  (σ : String → String)
+  (k : ℕ)
+  (x : String)
+  (h1 : σ x = x) :
+  Formula.sub_Var (str_fun_to_var_fun σ) (openFormulaAux k (free_ x) F) =
+    openFormulaAux k (free_ x) (Formula.sub_Var (str_fun_to_var_fun σ) F) :=
+  by
+  induction F generalizing k
+  case pred_ X xs =>
+    simp only [openFormulaAux]
+    simp only [Formula.sub_Var]
+    simp
+    simp only [List.map_eq_map_iff]
+    intro v _
+    exact SubOpenVar v σ k x h1
+  case not_ phi phi_ih =>
+    simp only [openFormulaAux]
+    simp only [Formula.sub_Var]
+    congr! 1
+    apply phi_ih
+  case imp_ phi psi phi_ih psi_ih =>
+    simp only [openFormulaAux]
+    simp only [Formula.sub_Var]
+    congr! 1
+    · apply phi_ih
+    · apply psi_ih
+  case forall_ phi phi_ih =>
+    simp only [openFormulaAux]
+    simp only [Formula.sub_Var]
+    congr! 1
+    apply phi_ih
+
+
+lemma SubCloseFormula
+  (F : Formula)
+  (σ : String → String)
+  (x : String)
+  (k : ℕ)
+  (h1 : σ x = x)
+  (h2 : ∀ (y : String), ¬ x = σ y) :
+  Formula.sub_Var (str_fun_to_var_fun σ) (closeFormulaAux (free_ x) k F) = closeFormulaAux (free_ x) k (Formula.sub_Var (str_fun_to_var_fun σ) F) :=
+  by
+  induction F generalizing k
+  case pred_ X xs =>
+    simp only [closeFormulaAux]
+    simp only [Formula.sub_Var]
+    simp
+    simp only [List.map_eq_map_iff]
+    intro v _
+    exact SubCloseVar v σ x k h1 h2
+  case not_ phi phi_ih =>
+    simp only [closeFormulaAux]
+    simp only [Formula.sub_Var]
+    congr! 1
+    apply phi_ih
+  case imp_ phi psi phi_ih psi_ih =>
+    simp only [closeFormulaAux]
+    simp only [Formula.sub_Var]
+    congr! 1
+    · apply phi_ih
+    · apply psi_ih
+  case forall_ phi phi_ih =>
+    simp only [closeFormulaAux]
+    simp only [Formula.sub_Var]
+    congr! 1
+    apply phi_ih
